compiler/src/examples/MMIO.v
@@ -10,7 +10,6 @@ Require Import compiler.FlatImp.
 Require Import riscv.util.ListLib.
 Require Import riscv.Decode.
 Require Import coqutil.sanity.
-Require Import riscv.Utility.
 Require Import riscv.MkMachineWidth.
 Require Import riscv.PseudoInstructions.
 Require Import riscv.InstructionCoercions.
@@ -26,59 +25,24 @@ Require Import compiler.Rem4.
 Require Import compiler.GoFlatToRiscv.
 Require Import compiler.SeparationLogic.
 Require Import coqutil.Datatypes.Option.
-
-
+Require Import coqutil.Z.HexNotation.
+Require Import compiler.Simp.
+Require Import compiler.util.Learning.
+Require Import compiler.SimplWordExpr.
+Require Import compiler.FlatToRiscv32.
 Import ListNotations.
-Existing Instance DefaultRiscvState.
-
-
-Module Type LEARNING.
-  Parameter Learnt: Prop -> Prop.
-  Parameter markLearnt: forall {P: Prop} (p: P), Learnt P.
-End LEARNING.
-
-Module Import Learning: LEARNING.
-  Definition Learnt(P: Prop) := P.
-  Definition markLearnt{P: Prop}(p: P): Learnt P := p.
-End Learning.
-
-Ltac learn_tac p H :=
-  let P := type of p in
-  lazymatch goal with
-  | H: Learnt P |- _ => fail
-  | |- _ =>
-    let L := fresh "L" in
-    pose proof (markLearnt p) as L; (* will stay around *)
-    pose proof p as H (* will likely be destructed *)
-  end.
-
-Tactic Notation "learn" constr(p) := let H := fresh in learn_tac p H.
-Tactic Notation "learn" constr(p) "as" ident(H) := learn_tac p H.
-
-Ltac cheap_saturate :=
-  unshelve (repeat match goal with
-    | H: _ /\ _ |- _ => let Hl := fresh H "l" in let Hr := fresh H "r" in destruct H as [Hl Hr]
-    | E: exists y, _ |- _ => let yf := fresh y in destruct E as [yf E]
-    | H: forall (x: ?T), _ |- _ =>
-      match type of T with
-      | Prop => fail 1
-      | _ => let x' := fresh x in (evar (x': T)); specialize (H x'); subst x'
-      end
-    | H1: _, H2: _ -> _ |- _ => let H3 := fresh H1 "_" H2 in learn (H2 H1) as H3
-  end);
-  [eauto..|].
 
 
 Open Scope ilist_scope.
 
-Definition var: Type := Z.
-Definition func: Type := Empty_set.
+Definition varname: Type := Z.
+Definition funname: Type := Empty_set.
 
-Instance act_dec: DecidableEq MMIOAction.
+Instance actname_eq_dec: DecidableEq MMIOAction.
 intros a b. destruct a; destruct b; (left + right); congruence.
 Defined.
 
-Definition compile_ext_call(results: list var)(a: MMIOAction)(args: list var):
+Definition compile_ext_call(results: list varname)(a: MMIOAction)(args: list varname):
   list Instruction :=
   match a with
   | MMInput =>
@@ -93,41 +57,95 @@ Definition compile_ext_call(results: list var)(a: MMIOAction)(args: list var):
     end
   end.
 
-Instance myparams: Syntax.parameters := {|
-  Syntax.varname := var;
-  Syntax.funname := func;
+Lemma compile_ext_call_length: forall binds f args,
+    Zlength (compile_ext_call binds f args) <= 1.
+Proof.
+  intros. unfold compile_ext_call.
+  destruct f; destruct binds; try destruct binds;
+  try destruct args; try destruct args; try destruct args;
+  cbv; intros; discriminate.
+Qed.
+
+Lemma compile_ext_call_emits_valid: forall iset binds a args,
+    Forall valid_register binds ->
+    Forall valid_register args ->
+    valid_instructions iset (compile_ext_call binds a args).
+Proof.
+  intros.
+  destruct a; destruct args; try destruct args; try destruct args;
+    destruct binds; try destruct binds;
+    intros instr HIn; simpl in *; intuition idtac; try contradiction.
+  - rewrite <- H1.
+    simp_step.
+    simp_step.
+    simp_step.
+    simp_step.
+    (* try simp_step. (* TODO this should not fail fatally *) *)
+    split; [|cbv;auto].
+    unfold Encode.respects_bounds. simpl.
+    unfold Encode.verify_I, valid_register, opcode_LOAD, funct3_LW in *.
+    repeat split; (lia || assumption).
+  - rewrite <- H1.
+    simp_step.
+    simp_step.
+    (* try simp_step. (* TODO this should not fail fatally *) *)
+    split; [|cbv;auto].
+    unfold Encode.respects_bounds. simpl.
+    unfold Encode.verify_S, valid_register, opcode_STORE, funct3_SW in *.
+    repeat split; (lia || assumption).
+Qed.
+
+Instance mmio_syntax_params: Syntax.parameters := {|
+  Syntax.varname := varname;
+  Syntax.funname := funname;
   Syntax.actname := MMIOAction;
 |}.
 
 Module Import MMIO.
   Class parameters := {
-    W :> Words;
+    byte :> Word.Interface.word 8;
+    byte_ok :> word.ok byte;
+    word :> Word.Interface.word 32;
+    word_ok :> word.ok word;
     mem :> map.map word byte;
     mem_ok :> map.ok mem;
-    locals :> map.map var word;
+    locals :> map.map varname word;
     locals_ok :> map.ok locals;
-    env :> map.map func (list var * list var * Syntax.cmd.cmd);
-    env_ok :> map.ok env;
   }.
 End MMIO.
 
 Section MMIO1.
   Context {p: unique! MMIO.parameters}.
 
-  Definition magicMMIOAddrLit: Z := 65524.
-  Definition simple_isMMIOAddr: word -> bool := word.eqb (word.of_Z magicMMIOAddrLit).
+  Lemma cases32: 32 = 32 \/ 32 = 64. lia. Qed.
 
-  Instance semantics_params: Semantics.parameters := {|
-    Semantics.syntax := myparams;
-    Semantics.width := width;
-    Semantics.funname_eqb f := Empty_set_rect _;
+  Instance Words32: Utility.Words := {
+    Utility.byte := byte;
+    Utility.word := word;
+    Utility.width_cases := cases32;
+  }.
+
+  (* Using the memory layout of FE310-G000 *)
+  Definition isGPIO0(addr: word): Prop := Ox"10012000" <= word.unsigned addr < Ox"10013000".
+  Definition isQSPI1(addr: word): Prop := Ox"10024000" <= word.unsigned addr < Ox"10025000".
+  Definition isMMIOAddr(addr: word): Prop :=
+    word.unsigned addr mod 4 = 0 /\ (isGPIO0 addr \/ isQSPI1 addr).
+
+  Lemma loadWord_in_MMIO_is_None: forall (m: mem) (addr: word),
+      map.undef_on m isMMIOAddr ->
+      isMMIOAddr addr ->
+      Memory.loadWord m addr = None.
+  Proof.
+  Admitted.
+
+  Instance mmio_semantics_params: Semantics.parameters := {|
+    Semantics.syntax := mmio_syntax_params;
+    Semantics.width := 32;
+    Semantics.funname_eqb := Empty_set_rect _;
     Semantics.ext_spec t m action (argvals: list word) (post: (mem -> list word -> Prop)) :=
       match argvals with
       | addr :: _ =>
-        simple_isMMIOAddr addr = true /\
-        (* TODO this one says "exists addr in the 4-byte range which is undefined", but we probably
-           need "forall addr in the 4 byte range, it is undefined" *)
-        Memory.loadWord m addr = None /\ (* <-- TODO move to ext_guarantee *)
+        isMMIOAddr addr /\
         match action with
         | MMInput => argvals = [addr] /\ forall val, post m [val]
         | MMOutput => exists val, argvals = [addr; val] /\ post m nil
@@ -136,206 +154,122 @@ Section MMIO1.
       end;
   |}.
 
-Instance compilation_params: FlatToRiscvDef.parameters. refine ({|
-  FlatToRiscvDef.actname := MMIOAction;
-  FlatToRiscvDef.compile_ext_call := compile_ext_call;
-  FlatToRiscvDef.max_ext_call_code_size _ := 1;
-|}).
-  intros. unfold compile_ext_call.
-  destruct f; destruct binds; try destruct binds;
-  try destruct args; try destruct args; try destruct args;
-  cbv; intros; discriminate.
-Defined.
+  Instance compilation_params: FlatToRiscvDef.parameters := {
+    FlatToRiscvDef.actname := MMIOAction;
+    FlatToRiscvDef.compile_ext_call := compile_ext_call;
+    FlatToRiscvDef.max_ext_call_code_size _ := 1;
+    FlatToRiscvDef.compile_ext_call_length := compile_ext_call_length;
+    FlatToRiscvDef.compile_ext_call_emits_valid := compile_ext_call_emits_valid;
+  }.
 
-(*
-addr = magicMMIOAddr;
-loop {
-  i = input addr;
-  stay in loop only if i is non-zero;
-  s = i * i;
-  output addr s;
-}
-*)
+  Section CompilationTest.
+    Definition magicMMIOAddrLit: Z := Ox"10024000".
+    Variable addr: varname.
+    Variable i: varname.
+    Variable s: varname.
 
-Definition _addr: Syntax.varname := 1.
-Definition _i: Syntax.varname := 2.
-Definition _s: Syntax.varname := 3.
+    (*
+    addr = magicMMIOAddr;
+    loop {
+      i = input addr;
+      stay in loop only if i is non-zero;
+      s = i * i;
+      output addr s;
+    }
+    *)
+    Definition squarer: stmt :=
+      (SSeq (SLit addr magicMMIOAddrLit)
+            (SLoop (SLoad Syntax.access_size.four i addr)
+                   (CondNez i)
+                   (SSeq (SOp s Syntax.bopname.mul i i)
+                         (SStore Syntax.access_size.four addr s)))).
 
-Definition squarer: stmt :=
-  (SSeq (SLit _addr magicMMIOAddrLit)
-        (SLoop (SLoad Syntax.access_size.four _i _addr)
-               (CondNez _i)
-               (SSeq (SOp _s Syntax.bopname.mul _i _i)
-                     (SStore Syntax.access_size.four _addr _s)))).
+    Definition compiled: list Instruction := Eval cbv in compile_stmt RV32IM squarer.
+    Print compiled.
+  End CompilationTest.
 
-Definition compiled: list Instruction := Eval cbv in compile_stmt RV32IM squarer.
+  Arguments LittleEndian.combine: simpl never. (* TODO can we put this next to its definition? *)
+  Arguments mcomp_sat: simpl never.
 
-Print compiled.
+  Instance FlatToRiscv_params: FlatToRiscv.parameters := {
+    FlatToRiscv.def_params := compilation_params;
+    FlatToRiscv.locals := locals;
+    FlatToRiscv.mem := (@mem p);
+    FlatToRiscv.MM := OStateND_Monad _;
+    FlatToRiscv.RVM := IsRiscvMachineL;
+    FlatToRiscv.PRParams := MinimalMMIOPrimitivesParams;
+    FlatToRiscv.ext_spec := ext_spec;
+    FlatToRiscv.ext_guarantee mach := map.undef_on mach.(getMem) isMMIOAddr;
+  }.
 
-Lemma option_all_singleton: forall {A: Type} (a: A) (l: list (option A)),
-    List.option_all l = Some [a] ->
-    l = [Some a].
-Proof.
-  intros.
-  destruct l; [|destruct l]; simpl in *; inversion H; destruct o; try congruence.
-  destruct o0; destruct (List.option_all l); discriminate.
-Qed.
+  Instance assume_riscv_word_properties: RiscvWordProperties.word.riscv_ok word. Admitted.
 
-Lemma map_singleton: forall {A B: Type} (f: A -> B) (l: list A) (b: B),
-    List.map f l = [b] ->
-    exists a, l = [a] /\ f a = b.
-Proof.
-  intros. destruct l; [|destruct l]; simpl in *; try discriminate; inversion H; eauto.
-Qed.
+  Ltac contrad := contradiction || discriminate || congruence.
 
-Lemma Forall_singleton: forall {A: Type} (P: A -> Prop) (a: A),
-    Forall P [a] ->
-    P a.
-Proof.
-  intros. inversion H. assumption.
-Qed.
-
-Arguments Z.mul: simpl never.
-
-Ltac head e :=
-  match e with
-  | ?f _ => head f
-  | _ => e
-  end.
-
-Definition protected(P: Prop) := P.
-
-Ltac protect_equalities :=
-  repeat match goal with
-         | H: ?a = ?b |- _ => change (protected (a = b)) in H
-         end.
-
-Ltac unprotect_equalities :=
-  repeat match goal with
-         | H: protected (?a = ?b) |- _ => change (a = b) in H
-         end.
-
-Ltac invert_hyp H := protect_equalities; inversion H; clear H; subst; unprotect_equalities.
-
-Ltac invert_ind name :=
-  match goal with
-  | H: ?P |- _ =>
-    let h := head P in constr_eq h name;
-    invert_hyp H
-  end.
-
-Ltac destruct_unique_match :=
-  let contrad := (exfalso; (contradiction || discriminate || congruence)) in
-  match goal with
-  | H: context[match ?e with _ => _ end] |- _ =>
-    is_var e;
-    destruct e;
-    try contrad;
-    let n := numgoals in guard n <= 1
-  | H: context[match ?e with _ => _ end] |- _ =>
-    let E := fresh "E" in destruct e eqn: E;
-    try contrad;
-    let n := numgoals in guard n <= 1
-  end.
-
-Ltac destruct_unique_matches := repeat destruct_unique_match.
-
-Ltac contrad := contradiction || discriminate || congruence.
-
-Arguments LittleEndian.combine: simpl never. (* TODO can we put this in word interface? *)
-Arguments mcomp_sat: simpl never.
-
-Definition TODO{T: Type}: T. Admitted.
-
-Instance FlatToRiscv_params: FlatToRiscv.parameters := {|
-  FlatToRiscv.def_params := compilation_params;
-  FlatToRiscv.locals := locals;
-  FlatToRiscv.mem := (@mem p);
-  FlatToRiscv.MM := OStateND_Monad _;
-  FlatToRiscv.RVM := IsRiscvMachineL;
-  FlatToRiscv.PRParams := MinimalMMIOPrimitivesParams;
-  FlatToRiscv.ext_spec := ext_spec;
-  FlatToRiscv.ext_guarantee := TODO;
-|}.
-
-Set Refine Instance Mode.
-
-Instance FlatToRiscv_hyps: FlatToRiscv.assumptions.
-Proof.
-econstructor. all: try typeclasses eauto.
-- apply TODO.
-- apply TODO.
-- intros initialL action.
-  destruct initialL as [initialRegs initialPc initialNpc initialMem initialLog].
-  destruct action; cbv [getRegs getPc getNextPc getMem getLog]; intros.
-  + (* MMInput *)
-    simpl in *|-.
-    invert_ind @exec; [].
-    simpl in *|-.
-    repeat match goal with
-           | l: list _ |- _ => destruct l;
-                                 try (exfalso; (contrad || (cheap_saturate; contrad))); []
-           end.
-    destruct argvars; [| solve [exfalso; simpl in *; repeat destruct_unique_match] ].
-    simpl in *|-.
-    destruct_unique_match.
-    replace r2 with r in * by congruence.
-    destruct_products.
-    repeat match goal with
-           | H: Forall _ _ |- _ => apply Forall_singleton in H
-           end.
-    subst.
-    eapply runsToNonDet.runsToStep; cycle 1.
-    * intro mid.
-      apply id.
-    * eapply go_fetch_inst; [reflexivity| | |].
-      { simpl in *. ecancel_assumption. }
-      { unfold valid_register in *.
-        cbv -[Z.lt Z.le]; repeat split; auto; try lia. }
-      cbv [Execute.execute ExecuteI.execute].
-      rewrite associativity.
-      eapply go_getRegister; [eassumption..|]. rewrite associativity.
-      cbv [getRegs].
-      match goal with
-      | |- context [?T] =>
-        match T with
-        | translate Load ?w ?a => replace T with (Return a)
-        end
-      end.
-      {
-      rewrite left_identity. rewrite associativity.
-      rename r into addr.
-      replace (add addr (ZToReg 0)) with addr by apply TODO.
-      apply spec_Bind.
-      refine (ex_intro _ (fun v m => m = _) _).
-      split.
-      - apply spec_loadWord. simpl. right. repeat split; try assumption.
-        (* TODO use ext_guarantee here *) admit.
-      - intros. subst. apply go_setRegister; [assumption|].
-        apply go_step.
-        apply runsToDone.
-        simpl.
-        repeat split.
-        + unfold mmioLoadEvent.
-          specialize (H16 initialMem [signedByteTupleToReg a]).
-          destruct H16 as [ l' [A B] ].
-          { (* TODO trace translation *) admit. }
-          { inversion_option.
-            subst l'.
-            Fail exact B.
-            (* TODO trace translation *) admit. }
-        + rewrite Zlength_cons, Zlength_nil. apply TODO. (* TODO word solver *)
-        + rewrite Zlength_cons, Zlength_nil. apply TODO. (* TODO word solver *)
-        + simpl in *. seplog.
-        + admit. (* prove ext_guarantee preservation *)
-      }
-      { reflexivity. }
-  + (* MMOutput *)
-    apply TODO.
-  - (* go_load *)
-    apply TODO.
-  - (* go_store *)
-    apply TODO.
-  Admitted.
+  Instance FlatToRiscv_hyps: FlatToRiscv.assumptions.
+  Proof.
+    constructor. all: try typeclasses eauto.
+    - (* ext_guarantee preservable: *)
+      simpl. unfold map.same_domain, map.sub_domain, map.undef_on, map.agree_on in *.
+      intros. destruct H0 as [A B].
+      specialize H with (1 := H2).
+      rewrite map.get_empty in *.
+      destruct (map.get (getMem m2) k) eqn: E; [exfalso|reflexivity].
+      edestruct B; [eassumption|]. congruence.
+    - (* compile_ext_call_correct *)
+      intros *. intros ? ? V_argvars V_resvars. intros.
+      pose proof (compile_ext_call_emits_valid FlatToRiscv.iset _ action _ V_resvars V_argvars).
+      destruct initialL as [initialRegs initialPc initialNpc initialMem initialLog].
+      destruct action; cbv [getRegs getPc getNextPc getMem getLog] in *.
+      + (* MMInput *)
+        simpl in *|-.
+        simp.
+        simpl in *|-.
+        repeat match goal with
+               | l: list _ |- _ => destruct l;
+                                     try (exfalso; (contrad || (cheap_saturate; contrad))); []
+               end.
+        simp.
+        destruct argvars; cycle 1. {
+          exfalso. rename H9 into A. clear -A. simpl in *. simp.
+          destruct_one_match_hyp; congruence.
+        }
+        simpl in *|-.
+        simp.
+        subst insts.
+        eapply runsToNonDet.runsToStep; cycle 1.
+        * intro mid.
+          apply id.
+        * simulate_step.
+          simulate_step.
+          simulate_step.
+          simulate_step.
+          simulate_step.
+          simulate_step.
+          simpl_word_exprs word_ok.
+          apply spec_Bind.
+          refine (ex_intro _ (fun v m => m = _) _).
+          split.
+          { apply spec_loadWord. simpl. right. repeat split; try assumption.
+            apply loadWord_in_MMIO_is_None; assumption. }
+          { intros. subst. simulate. simpl. apply runsToNonDet.runsToDone.
+            simpl.
+            repeat split; try assumption.
+              specialize (H15 initialMem [signedByteTupleToReg a]).
+              destruct H15 as [ l' [A B] ].
+              { specialize (H8 (signedByteTupleToReg a)).
+                Fail exact H8. (* TODO trace translation *) apply TODO. }
+              { inversion_option.
+                subst l'.
+                unfold mmioLoadEvent, signedByteTupleToReg in *. simpl in *.
+                Fail exact B. (* TODO trace translation *) apply TODO. } }
+      + (* MMOutput *)
+        apply TODO.
+      - (* go_load *)
+        (* TODO make FlatToRiscv32.parameters and eapply go_load *)
+        apply TODO.
+      - (* go_store *)
+        apply TODO.
+  Qed.
 
 End MMIO1.
