compiler/src/GoFlatToRiscv.v
@@ -240,7 +240,7 @@ Ltac sidecondition :=
   | |- _ => reflexivity
   (* but we don't have a general "eassumption" branch, only "assumption": *)
   | |- _ => assumption
-  | H: valid_instructions _ _ |- Encode.verify _ _ =>
+  | H: FlatToRiscvDef.valid_instructions _ _ |- Encode.verify _ _ =>
     apply H; clear; eauto 10 using in_cons, in_or_app, in_eq
   | |- Memory.load ?sz ?m ?addr = Some ?v =>
     simpl; unfold Memory.load, Memory.load_Z;
