compiler/src/util/Learning.v
@@ -1,0 +1,35 @@
+Module Type LEARNING.
+  Parameter Learnt: Prop -> Prop.
+  Parameter markLearnt: forall {P: Prop} (p: P), Learnt P.
+End LEARNING.
+
+Module Import Learning: LEARNING.
+  Definition Learnt(P: Prop) := P.
+  Definition markLearnt{P: Prop}(p: P): Learnt P := p.
+End Learning.
+
+Ltac learn_tac p H :=
+  let P := type of p in
+  lazymatch goal with
+  | H: Learnt P |- _ => fail
+  | |- _ =>
+    let L := fresh "L" in
+    pose proof (markLearnt p) as L; (* will stay around *)
+    pose proof p as H (* will likely be destructed *)
+  end.
+
+Tactic Notation "learn" constr(p) := let H := fresh in learn_tac p H.
+Tactic Notation "learn" constr(p) "as" ident(H) := learn_tac p H.
+
+Ltac cheap_saturate :=
+  unshelve (repeat match goal with
+    | H: _ /\ _ |- _ => let Hl := fresh H "l" in let Hr := fresh H "r" in destruct H as [Hl Hr]
+    | E: exists y, _ |- _ => let yf := fresh y in destruct E as [yf E]
+    | H: forall (x: ?T), _ |- _ =>
+      match type of T with
+      | Prop => fail 1
+      | _ => let x' := fresh x in (evar (x': T)); specialize (H x'); subst x'
+      end
+    | H1: _, H2: _ -> _ |- _ => let H3 := fresh H1 "_" H2 in learn (H2 H1) as H3
+  end);
+  [eauto..|].
